in the progress of porting bedrock files.

src/DiscreteMemory.v
@@ -19,7 +19,7 @@ Module DiscreteHeap (B : Memory)
 
   Instance EqDec_addr : EquivDec.EqDec addr (@eq addr) := addr_dec.
 
-  Definition smem' dom : Type := hlist (fun _ : addr => option value) dom.
+  Definition smem' dom : Type := hlist (fun _ : addr => option value)%type dom.
 
   Fixpoint smem_emp' (ls : list addr) : smem' ls :=
     match ls with
@@ -116,9 +116,12 @@ Module DiscreteHeap (B : Memory)
 
   Definition models (m : smem) (m' : B.mem) : Prop :=
     models' _ m m'.
-(*
-  Definition relevant (sm : smem) := relevant' _ sm.
-*)
+
+  Definition in_domain p m : Prop :=
+    (smem_get p m = None) -> False.
+
+  Definition same_domain m1 m2 : Prop :=
+    forall p, in_domain p m1 <-> in_domain p m2.
 
   Theorem Reflexive_eqv : Reflexive smem_eqv.
   Proof. intuition. Qed.
@@ -197,55 +200,33 @@ Module DiscreteHeap (B : Memory)
       destruct (hlist_hd d); auto. }
   Qed.
 
+  Theorem split_in_domain : forall a b c,
+    split a b c ->
+      forall p, in_domain p a <-> (in_domain p b \/ in_domain p c).
+  Proof.
+    unfold split, join, disjoint, in_domain, smem_get, smem.
+    generalize BD.all_addr; induction l; simpl in *; intros.
+    intuition.
+    destruct (addr_dec a p); subst.
+    { intuition. rewrite H0 in *. subst; simpl in *; auto. 
+      rewrite H0 in *. subst. simpl in *; auto.
+      rewrite H0 in *; subst. destruct (hlist_hd b); auto.
+      destruct (hlist_hd b); auto. subst; simpl in *; auto. }
+    { destruct H. destruct H. subst. simpl in *. eauto. }
+  Qed.      
+
   Theorem smem_get_sound : forall s m,
     models s m ->
     forall a v, smem_get a s = Some v ->
                 M.mem_get m a = Some v.
   Proof.
-  Admitted.
-
-  Theorem smem_set_sound : forall s m,
-    models s m ->
-    forall a v s', smem_set a v s = Some s' ->
-    exists m', M.mem_set m a v = Some m' /\ models s' m'. 
-  Proof.
-  Admitted.
-
-  (** memoryIn **)
-  Section memoryIn.
-    Variable m : mem.
-
-    Fixpoint memoryIn' (ls : list addr) : smem' ls :=
-      match ls with 
-        | nil => HNil
-        | l :: ls => HCons (mem_get m l) (memoryIn' ls)
-      end. 
-
-    Definition memoryIn : smem := memoryIn' BD.all_addr.
-  End memoryIn.
-
-  Theorem memoryIn_sound : forall m, 
-    models (memoryIn m) m.
-  Proof.
-    unfold models, memoryIn. generalize BD.all_addr.
-    induction l; simpl; auto.
-    intuition. destruct (mem_get m a); auto.
-  Qed.
-
-End DiscreteHeap.
-
-Export Heaps.
-
-(*
-  Local Hint Resolve mem_get_set_eq mem_get_set_neq : memory.
-
-  Lemma smem_set_not_in : forall l m p v,
-    ~In p l -> smem_set' l p v m = None.
-  Proof.
-    induction l; simpl; auto.
-      intros.
-      destruct (addr_dec a p); subst; intuition.
-      rewrite IHl; auto.
+    unfold models, smem_get, mem_get, smem.
+    generalize BD.all_addr. induction l; simpl in *; intros; try congruence.
+    rewrite hlist_eta with (h := s) in H; eauto with typeclass_instances.
+    simpl in *; intuition.
+    destruct (addr_dec a a0); subst.
+    rewrite H0 in *; auto.
+    intuition eauto.
   Qed.
 
   Ltac simp ext :=
@@ -288,17 +269,8 @@ Export Heaps.
         | [ H : _ /\ _ |- _ ] => destruct H
         | [ |- _ ] => congruence
         | [ |- _ ] => ext
-      end; simpl in * ); eauto 10 with memory.
+      end; simpl in * ).
 
-  Theorem satisfies_get : forall m m',
-    models m m' ->
-    forall p v, 
-      smem_get p m = Some v ->
-      mem_get m' p = Some v.
-  Proof.
-    unfold models, smem_get, smem.
-    induction BD.all_addr; simp intuition. 
-  Qed.
 
   Lemma models_set_not_in : forall l m sm p v,
     models' l sm m ->
@@ -309,258 +281,109 @@ Export Heaps.
     induction l; try solve [ simp intuition ].
       simp auto.
       destruct (addr_dec a p); destruct (in_dec addr_dec p l); subst; try solve [ intuition ].
-
-      split; eauto. rewrite <- H3. eapply B.mem_get_set_neq; eauto.
+      split; eauto. erewrite B.mem_get_set_neq; eauto. 
+      split; eauto. 
   Qed.
 
-  Local Hint Resolve models_set_not_in : memory.
-
-  Theorem models_set : forall sm m,
-    models sm m ->
-    forall p v sm',
-      smem_set p v sm = Some sm' ->
-      exists m',
-      mem_set m p v = Some m' /\ models sm' m'.
+  Lemma smem_set_same_domain : forall s,
+    forall a v s', smem_set a v s = Some s' ->
+    same_domain s s'.
   Proof.
-    unfold models, smem_set, smem_get, smem.
     generalize BD.NoDup_all_addr.
-    induction BD.all_addr; simp auto.
-    { 
-
-
-      destruct (proj1 (mem_set_acc _ _) H2 v). rewrite H3. eexists; split; eauto.        
-      erewrite mem_get_set_eq; eauto with memory.
-
-      Focus.
-      eapply IHl in H1; eauto.
-      destruct H1; eexists; intuition; eauto with memory.
-      erewrite mem_get_set_neq; eauto.
-
-      Focus.
-      eapply IHl in H1; eauto. destruct H1; eexists; intuition eauto.
+    unfold models, same_domain, in_domain, smem_set, smem_get, smem.
+    generalize BD.all_addr. induction l; simpl in *; intros; try congruence.
+    destruct (addr_dec a a0); subst.
+    { destruct (hlist_hd s); try congruence. inversion H0; clear H0; subst; simpl in *.
+      destruct (addr_dec a0 p); auto. intuition try congruence. intuition. }
+    { revert H0. case_eq (smem_set' l a0 v (hlist_tl s)); intros; try congruence.
+      inversion H1; clear H1; subst; simpl in *.
+      destruct (addr_dec a p). intuition. eapply IHl. inversion H; auto. eauto. }
   Qed.
 
-  Lemma smem_set_get_neq : forall p m m' a b,
-    smem_set a b m = Some m' ->
-    a <> p ->
-    smem_get p m' = smem_get p m.
+  Theorem smem_set_sound' : forall s m,
+    models s m ->
+    forall a v s', smem_set a v s = Some s' ->
+    exists m', M.mem_set m a v = Some m' /\ models s' m'. 
   Proof.
-    unfold smem, smem_get, smem_set.
-    induction BD.all_addr; simp intuition.
+    generalize BD.NoDup_all_addr.
+    unfold models, smem_set, mem_get, smem.
+    generalize BD.all_addr. induction l; simpl in *; intros; try congruence.
+    rewrite hlist_eta with (h := s) in H0; eauto with typeclass_instances.
+    simpl in *; intuition.
+    destruct (addr_dec a a0); subst.
+    { destruct (hlist_hd s); try congruence.
+      inversion H1; clear H1; subst.
+      simpl in *.
+      case_eq (mem_set m a0 v); intros. eexists; split; eauto.
+      intuition; eauto using B.mem_get_set_eq.
+      eapply models_set_not_in; eauto.
+      inversion H; auto.
+      
+      exfalso. eapply mem_get_mem_set; eauto. congruence. }
+
+    { revert H1.
+      case_eq (smem_set' l a0 v (hlist_tl s)); intros.
+      inversion H1; clear H1; subst. eapply IHl in H0; eauto.
+      destruct H0. simpl. eexists; intuition eauto. 
+      destruct (hlist_hd s); auto.
+      erewrite mem_get_set_neq; eauto. inversion H; auto. 
+      
+      congruence. }
   Qed.
 
-  Lemma smem_set_get_eq : forall m m' a b,
-    smem_set a b m = Some m' ->
-    smem_get a m' = Some b.
+  Theorem smem_set_sound : forall s m,
+    models s m ->
+    forall a v s', smem_set a v s = Some s' ->
+    same_domain s s' /\
+    exists m', M.mem_set m a v = Some m' /\ models s' m'. 
   Proof.
-    unfold smem, smem_get, smem_set.
-    induction BD.all_addr; simp intuition.
+    intuition eauto using smem_set_sound', smem_set_same_domain.
   Qed.
 
-  Lemma split_smem_get : forall a b c p v,
+
+  Theorem split_smem_get : forall a b c p v,
     split a b c ->
-      (smem_get p b = Some v \/ smem_get p c = Some v) ->
+      smem_get p b = Some v ->
       smem_get p a = Some v.
   Proof.
-    unfold smem, split, disjoint, join, smem_get, smem.
-    induction BD.all_addr; simp intuition.
+    unfold models, smem_get, mem_get, smem, split, disjoint, join, smem.
+    generalize BD.all_addr. induction l; simpl in *; intros; try congruence.
+    destruct (addr_dec a p); subst.
+    { intuition; subst; simpl; rewrite H0; auto. }
+    { intuition; subst; simpl; try rewrite H1; eauto. }
   Qed.
 
-  Lemma smem_set_get_valid : forall m p v v',
-    smem_get p m = Some v' ->
-    smem_set p v m <> None.
+  Theorem split_smem_set : forall a b c p v b',
+    split a b c ->
+      smem_set p v b = Some b' ->
+      exists a', split a' b' c /\
+        smem_set p v a = Some a'.
   Proof.
-    unfold smem_get, smem_set, smem.
-    induction BD.all_addr; simp intuition.
+    unfold models, smem_set, mem_set, smem, split, disjoint, join, smem.
+    generalize BD.all_addr. induction l; simpl in *; intros; try congruence.
+    destruct (addr_dec a p); subst.
+    { intuition; subst; simpl in *; rewrite H1 in *; try congruence.
+      destruct (hlist_hd b); try congruence; simpl in *. inversion H0; clear H0; subst; simpl in *.
+      eexists. intuition eauto. }
+    { revert H0; case_eq (smem_set' l p v (hlist_tl b)); intros; try congruence.
+      inversion H1; clear H1; subst. simpl in *.
+      intuition; subst; simpl in *; try rewrite H1 in *.
+      eapply IHl in H0; eauto.
+      destruct H0; intuition; subst. rewrite H2. eexists; eauto.
+
+      eapply IHl in H0; eauto. destruct H0. intuition.
+      subst. rewrite H2. eexists; intuition eauto. }
   Qed.
 
-  Lemma split_set : forall a b,
-    disjoint a b ->
-    forall p v a',
-    smem_set p v a = Some a' ->
-      disjoint a' b /\ 
-      smem_set p v (join a b) = Some (join a' b).
+  Global Instance Symetric_same_domain : Symmetric same_domain.
+  Proof. clear; red; firstorder. Qed.
+
+  Global Instance Trans_same_domain : Transitive same_domain.
   Proof.
-    unfold smem, disjoint, join, smem_set, smem.
-    induction BD.all_addr; simpl; intros; try congruence.
-      destruct (addr_dec a p); subst.
-      destruct H. destruct H; rewrite H in *; try congruence.
-        destruct (hlist_hd a0); try congruence.
-        inversion H0; auto.
-
-      generalize dependent H0.
-      case_eq (smem_set' l p v (hlist_tl a0)); intros; try congruence.
-        inversion H1; clear H1; subst.
-        eapply IHl in H0. 2: destruct H; eauto.
-        simp intuition.
+    clear.
+    red. unfold same_domain. firstorder.
   Qed.
-
-
-  Ltac unfold_all :=
-    unfold smem, split, join, disjoint, smem_emp, semp; 
-    unfold smem, split, join, disjoint, smem_emp, semp.
-  Ltac break :=
-    simpl; intros; try reflexivity;
-      repeat (simpl in *; match goal with
-                            | [ H : HCons _ _ = HCons _ _ |- _ ] =>
-                              inversion H; clear H
-                            | [ H : _ /\ _ |- _ ] => destruct H
-                            | [ H : @existT _ _ _ _ = @existT _ _ _ _ |- _ ] => 
-                              eapply (@Eqdep_dec.inj_pair2_eq_dec _ (list_eq_dec B.addr_dec)) in H
-                            | [ H : @existT _ _ _ _ = @existT _ _ _ _ |- _ ] => 
-                              eapply (@Eqdep_dec.inj_pair2_eq_dec _ B.addr_dec) in H
-                            | [ H : _ = _ |- _ ] => rewrite H in *
-                          end).
-  
-  Lemma disjoint_join : forall a b, disjoint a b -> join a b = join b a.
-  Proof.
-    unfold_all; induction a; break; f_equal; intuition; subst.
-      destruct (hlist_hd b0); reflexivity.
-      rewrite H1. destruct b; reflexivity.
-  Qed.
-    
-  Lemma disjoint_comm : forall ml mr, disjoint ml mr -> disjoint mr ml.
-  Proof.
-    unfold_all; induction ml; break; intuition.
-  Qed.
-
-  Hint Resolve disjoint_join disjoint_comm : disjoint.
-
-  Lemma split_assoc' : forall b a c d e, split a b c -> split c d e ->
-    split a (join d b) e.
-  Proof.
-    unfold_all; induction b; break; eauto.
-    edestruct IHb. split; try eassumption. reflexivity. split; try eassumption.
-    reflexivity.
-    intuition; break; auto. destruct (hlist_hd d); auto.
-    destruct (hlist_hd d); try congruence.
-  Qed.
-
-  Lemma split_comm : forall m ml mr, split m ml mr -> split m mr ml.
-  Proof.
-    unfold_all. induction ml; break; eauto. edestruct IHml.
-    split; try eassumption. reflexivity. 
-    intuition; subst. rewrite H3. destruct (hlist_hd mr); auto.
-    rewrite H4. rewrite H3. destruct b; auto.
-  Qed.
-
-  Lemma disjoint_split_join : forall a b, disjoint a b -> split (join a b) a b.
-  Proof.
-    unfold split, disjoint; intros; intuition.
-  Qed.
-
-  Lemma split_split_disjoint : forall b a c d e,
-    split a b c -> split b d e -> disjoint c d.
-  Proof.
-    unfold_all. induction b; break. subst. split.
-    intuition; destruct (hlist_hd c); eauto. destruct (hlist_hd d); auto.
-    eapply IHb. split; auto. split; auto. auto.
-  Qed.
-
-  Lemma hlist_destruct : forall T (F : T -> Type) a b (m : hlist F (a :: b)),
-    exists A, exists B, m = HCons A B.
-  Proof.
-    intros.
-    refine (match m as m in hlist _ ls return
-              match ls as ls return hlist _ ls -> Type with
-                | nil => fun _ => unit
-                | a :: b => fun m => exists A : F a, exists B : hlist F b, m = HCons A B
-              end m
-              with
-              | HNil => tt
-              | HCons _ _ _ _ => _
-            end).
-    do 2 eexists; reflexivity.
-  Qed.
-  Lemma hlist_nil : forall T (F : T -> Type) (m : hlist F nil), m = HNil.
-  Proof.
-    intros. 
-    refine (match m as m in hlist _ ls return
-              match ls as ls return hlist _ ls -> Type with
-                | nil => fun m => m = HNil
-                | _ :: _ => fun _ => unit
-              end m
-              with
-              | HNil => _ 
-              | _ => tt
-            end). reflexivity.
-  Qed.
-
-  Lemma split_semp : forall b a c, 
-    split a b c -> semp b -> a = c.
-  Proof.
-    unfold_all. unfold semp, smem_emp. unfold_all.
-    induction b; simpl; intros; subst; auto.
-    rewrite hlist_nil. rewrite (hlist_nil _ _ a). reflexivity.
-    destruct (hlist_destruct _ _ _ _ a).
-    destruct (hlist_destruct _ _ _ _ c).
-    destruct H1. destruct H2. subst. specialize (IHb x2 x3).
-    rewrite IHb; break; intuition; auto.
-  Qed.
-
-  Lemma semp_smem_emp : semp smem_emp.
-  Proof.
-    unfold semp, smem_emp; auto.
-  Qed.
-
-  Lemma split_a_semp_a : forall a, 
-    split a smem_emp a.
-  Proof.
-    unfold_all. induction a; simpl; intuition. rewrite <- H0. reflexivity.
-  Qed.
-     
-  Lemma cons_not_in : forall T (a : T) b ls,
-    a :: b = ls ->
-    ~ In a ls ->
-    forall P, P.
-  Proof.
-    intros; subst. exfalso; eapply H0. firstorder.
-  Qed.
-  
-  Lemma relevant_in : forall a l b,
-    In a (relevant' l b) ->
-    In a l.
-  Proof.
-    induction l; auto; intros.
-      rewrite (hlist_eta _ b) in H. simpl in H.
-      destruct (hlist_hd b). destruct H. subst. firstorder.
-      simpl in *. right. eapply IHl; eauto.
-      right. eapply IHl; eauto.
-  Qed.
-
-  Lemma relevant_not_in : forall a l b,
-    ~In a l ->
-    ~In a (relevant' l b).
-  Proof.
-    intros. intro. eapply H. eapply relevant_in; eauto.
-  Qed.
-
-  Lemma relevant_eq : forall a b c,
-    relevant a = relevant b ->
-    models a c ->
-    models b c ->
-    a = b.
-  Proof.
-    unfold relevant, models, smem. generalize BD.NoDup_all_addr.
-    induction BD.all_addr; simpl; intros.
-      rewrite (hlist_nil_only _ a). rewrite (hlist_nil_only _ b); auto.
-
-      rewrite (hlist_eta _ a0) in *. rewrite (hlist_eta _ a0) in H1.
-      rewrite (hlist_eta _ b) in *. rewrite (hlist_eta _ b) in H2.
-      simpl in *.
-      destruct (hlist_hd a0); destruct (hlist_hd b); intuition.
-        rewrite H2 in H3. inversion H3; subst. inversion H0;  f_equal. eapply IHl; eauto.
-          inversion H; auto.
-
-        eapply cons_not_in. eassumption.
-        eapply relevant_not_in. inversion H; auto.
-
-        eapply cons_not_in. symmetry. eassumption.
-        eapply relevant_not_in. inversion H; auto.
-        
-        f_equal; eauto. inversion H. eapply IHl; eauto.
-  Qed.
-
+      
   (** memoryIn **)
   Section memoryIn.
     Variable m : mem.
@@ -574,169 +397,59 @@ Export Heaps.
     Definition memoryIn : smem := memoryIn' BD.all_addr.
   End memoryIn.
 
-  Theorem smem_set_relevant : forall p v sm sm',
-    smem_set p v sm = Some sm' ->
-    relevant sm = relevant sm'.
-  Proof.
-    unfold relevant, smem_set.
-    induction BD.all_addr; simpl; intros; auto.
-      destruct (addr_dec a p); subst; auto.
-      destruct (hlist_hd sm); try congruence.
-      inversion H; clear H; subst. simpl. reflexivity.
-
-      revert H. case_eq (smem_set' l p v (hlist_tl sm)); intros; try congruence.
-      inversion H0; clear H0; subst; simpl in *.
-      destruct (hlist_hd sm); eauto. f_equal; eauto.
-  Qed.
-
-
-  Theorem models_memoryIn : forall m, 
+  Theorem memoryIn_sound : forall m, 
     models (memoryIn m) m.
   Proof.
     unfold models, memoryIn. generalize BD.all_addr.
     induction l; simpl; auto.
-    intuition. destruct (mem_acc_dec m a).
-    generalize (proj1 (mem_get_acc _ _) H). intro. destruct H0. rewrite H0. auto.
-    case_eq (mem_get m a); intuition; auto.
-    eapply mem_get_acc. eauto.
+    intuition. destruct (mem_get m a); auto.
   Qed.
 
-  
-
-
-
-(*
-  Theorem smem_set_word_relevant : forall ex p v sm sm',
-    smem_set_word ex p v sm = Some sm' ->
-    relevant sm = relevant sm'.
+  Theorem smem_set_get_eq : forall m p v' m', 
+    smem_set p v' m = Some m' ->
+    smem_get p m' = Some v'.
   Proof.
-    unfold smem_set_word; intros.
-    destruct (footprint_w p) as [ [ [ ? ? ] ? ] ? ].
-    destruct (ex v) as [ [ [ ? ? ] ? ] ? ].
-    repeat match goal with
-             | [ H : match ?X with 
-                       | Some _ => _
-                       | None => _ 
-                     end = Some _ |- _ ] => revert H; case_eq X; intros; try congruence
-             | [ H : smem_set _ _ _ = Some _ |- _ ] => 
-               eapply smem_set_relevant in H
-           end.
-    congruence.
+    unfold smem_set, smem_get, smem.
+    generalize BD.all_addr. induction l; simpl in *; intros; try congruence.
+    
+    destruct (addr_dec a p); subst; auto. destruct (hlist_hd m); try congruence.
+    inversion H; clear H; subst. auto.
+    eapply IHl.
+    instantiate (1 := hlist_tl m).
+    destruct (smem_set' l p v' (hlist_tl m)); try congruence.
+    inversion H; clear H; subst. auto.
   Qed.
-*)
 
 
-(*
-  Definition smem_get_word (implode : B * B * B * B -> W) (p : addr) (m : smem)
-    : option W :=
-    let '(a,b,c,d) := footprint_w p in
-    match smem_get a m , smem_get b m , smem_get c m , smem_get d m with
-      | Some a , Some b , Some c , Some d =>
-        Some (implode (a,b,c,d))
-      | _ , _ , _ , _ => None
-    end.
-
-  Definition smem_set_word (explode : W -> B * B * B * B) (p : addr) (v : W)
-    (m : smem) : option smem :=
-    let '(a,b,c,d) := footprint_w p in
-    let '(av,bv,cv,dv) := explode v in
-    match smem_set d dv m with
-      | None => None 
-      | Some m => match smem_set c cv m with
-                    | None => None
-                    | Some m => match smem_set b bv m with
-                                  | None => None
-                                  | Some m => smem_set a av m
-                                end
-                  end
-    end.
-*)
-
-(*
-  Lemma split_set_word : forall a b,
-    disjoint a b ->
-    forall i p v a',
-    smem_set_word i p v a = Some a' ->
-      disjoint a' b /\ 
-      smem_set_word i p v (join a b) = Some (join a' b).
+  Theorem smem_set_get_neq : forall m p v' m', 
+    smem_set p v' m = Some m' ->
+    forall p', p <> p' ->
+      smem_get p' m' = smem_get p' m.
   Proof.
-    unfold smem_set_word.
-    intros. destruct (i v); simp fail. 
-    repeat match goal with
-      | [ H : smem_set _ _ _ = Some _ |- _ ] =>
-        eapply split_set in H; [ rewrite (proj2 H) | eauto ]
-    end; tauto.
+    unfold smem_set, smem_get, smem.
+    generalize BD.all_addr. induction l; simpl in *; intros; try congruence.
+    
+    destruct (addr_dec a p); subst; auto. destruct (hlist_hd m); try congruence.
+    inversion H; clear H; subst. destruct (addr_dec p p'); auto; try congruence.
+
+    revert H.
+    case_eq (smem_set' l p v' (hlist_tl m)); intros; try congruence.
+    inversion H1; clear H1; subst. simpl in *.
+    eapply IHl in H; eauto. rewrite H. auto.
   Qed.
-*)
 
-
-(*
-  Lemma smem_set_get_word_eq : forall i e m m' a b,
-    (forall x, i (e x) = x) ->
-    smem_set_word e a b m = Some m' ->
-    smem_get_word i a m' = Some b.
+  Theorem smem_get_set_valid : forall m p v,
+    smem_get p m <> None ->
+    smem_set p v m <> None.
   Proof.
-    unfold smem_get_word, smem_set_word; intros.
-    generalize (footprint_disjoint a).
-    generalize dependent H0. case_eq (e b). simp intuition.
-    specialize (H2 _ _ _ _ (refl_equal _)). simp intuition.
-    repeat ((erewrite smem_set_get_eq; [ | repeat rewrite smem_set_get_neq by auto; eassumption ])
-      || (erewrite smem_set_get_neq by eauto)). simp intuition.
-  Qed.
-*)
-
-(*
-  Lemma split_smem_get_word : forall i a b c p v,
-    split a b c ->
-      (smem_get_word i p b = Some v \/ smem_get_word i p c = Some v) ->
-      smem_get_word i p a = Some v.
-  Proof.
-    unfold smem_get_word. simp intuition;
-    repeat (erewrite split_smem_get by eauto); auto.
+    unfold smem_get, smem_set, smem.
+    generalize (BD.all_addr); induction l; simpl; intros; auto.
+    destruct (addr_dec a p); subst; auto.
+    destruct (hlist_hd m); congruence.
+    eapply IHl with (v := v) in H.
+    destruct (smem_set' l p v (hlist_tl m)); congruence.
   Qed.
 
-  Theorem models_set_word : forall sm m,
-    models sm m ->
-    forall e p v sm',
-      smem_set_word e p v sm = Some sm' ->
-      exists m',
-           mem_set_word addr mem footprint_w mem_set e p v m = Some m' 
-        /\ models sm' m'.
-  Proof.
-    unfold smem_set_word, mem_set_word, smem_get_word; intros.
-    simp intuition. destruct (e v); simp intuition.
-    repeat match goal with
-             | [ H : models _ _ |- _ ] => 
-               eapply models_set in H; eauto; destruct H as [ ? [ ? ? ] ]
-             | [ H : _ = _ |- _ ] => rewrite H
-           end.
-    exists x2. intuition eauto.
-  Qed.
-*)
+End DiscreteHeap.
 
-(*
-  Lemma smem_set_get_valid_word : forall i e m p v v',
-    smem_get_word i p m = Some v' ->
-    smem_set_word e p v m <> None.
-  Proof.
-    unfold smem_get_word, smem_set_word.
-    intros. generalize (footprint_disjoint p).
-    intros; destruct (e v); simp intuition;
-    specialize (H0 _ _ _ _ (refl_equal _)); simp intuition;
-    (eapply smem_set_get_valid; [ | eauto ];
-      repeat (erewrite smem_set_get_neq; [ | solve [ eauto ] | solve [ eauto ] ]); eauto).
-  Qed.
-*)
-
-(*
-  Theorem models_get_word : forall i m m',
-    models m m' ->
-    forall p v, 
-      smem_get_word i p m = Some v ->
-      mem_get_word addr mem footprint_w mem_get i p m' = Some v.
-  Proof.
-    unfold mem_get_word, smem_get_word; simp intuition.
-    repeat erewrite models_get by eauto. auto.
-  Qed.
-*)
-*)
+Export Heaps.
