src/Heaps.v
@@ -15,11 +15,14 @@ Module Type Memory.
     mem_set m p v' = Some m' ->
     mem_get m' p = Some v'.
 
-  (** mem_set only modifies p **)
+  (** mem_set only modifies p **)  
   Parameter mem_get_set_neq : forall m p v m', 
     mem_set m p v = Some m' ->
-    forall p', p <> p' ->
+    forall p', p <> p' -> 
       mem_get m' p' = mem_get m p'.
+
+  Parameter mem_get_mem_set : forall m p,
+    mem_get m p <> None -> forall v, mem_set m p v <> None.
 
   Parameter addr_dec : forall a b : addr, {a = b} + {a <> b}.
 
@@ -30,46 +33,22 @@ Module Type SeparationMemory.
 
   Parameter smem : Type.
 
-(*
-  Parameter smem_eqv : smem -> smem -> Prop.
-
-  Parameter Reflexive_eqv : Reflexive smem_eqv.
-  Parameter Symmetric_eqv : Symmetric smem_eqv.
-  Parameter Transitive_eqv : Transitive smem_eqv.
-*)
-
   Parameter models : smem -> M.mem -> Prop.
 
   Parameter memoryIn : M.mem -> smem.
-
-(*
-  Parameter models_respects : forall s s' m,
-    smem_eqv s s' -> (models s m <-> models s' m).
-*)
 
   Parameter smem_emp : smem.
 
   Parameter smem_get : M.addr -> smem -> option M.value.
 
-(*
-  Parameter smem_get_respects : forall a s s',
-    smem_eqv s s' -> smem_get a s = smem_get a s'.
-*)
-
   Parameter smem_set : M.addr -> M.value -> smem -> option smem.
 
-(*
-  Parameter smem_set_respects : forall a v s s',
-    smem_eqv s s' -> smem_set a v s = smem_set a v s'.
-*)
+  Parameter in_domain : M.addr -> smem -> Prop.
+
+  Definition same_domain (l r : smem) : Prop :=
+    forall p, in_domain p l <-> in_domain p r.
 
   Parameter split : smem -> smem -> smem -> Prop.
-
-(*
-  Parameter split_respects : forall s1 s1' s2 s2' s3 s3',
-    smem_eqv s1 s1' -> smem_eqv s2 s2' -> smem_eqv s3 s3' ->
-    (split s1 s2 s3 <-> split s1' s2' s3').
-*)
 
   Parameter split_comm : forall a b c,
     split a b c -> split a c b.
@@ -80,6 +59,10 @@ Module Type SeparationMemory.
   Parameter split_assoc : forall a b c d e,
     split a b c -> split b d e ->
     exists f, split a d f /\ split f e c.
+
+  Parameter split_in_domain : forall a b c,
+    split a b c ->
+    forall p, in_domain p a <-> (in_domain p b \/ in_domain p c).
 
   Parameter memoryIn_sound : forall m,
     models (memoryIn m) m.
@@ -92,7 +75,32 @@ Module Type SeparationMemory.
   Parameter smem_set_sound : forall s m,
     models s m ->
     forall a v s', smem_set a v s = Some s' ->
+    same_domain s s' /\
     exists m', M.mem_set m a v = Some m' /\ models s' m'.
+
+  Parameter smem_set_get_eq : forall m p v' m', 
+    smem_set p v' m = Some m' ->
+    smem_get p m' = Some v'.
+
+  Parameter smem_get_set_valid : forall m p v,
+    smem_get p m <> None ->
+    smem_set p v m <> None.
+
+  Parameter smem_set_get_neq : forall m p v' m', 
+    smem_set p v' m = Some m' ->
+    forall p', p <> p' ->
+      smem_get p' m' = smem_get p' m.
+
+  Parameter split_smem_get : forall a b c p v,
+    split a b c ->
+      smem_get p b = Some v ->
+      smem_get p a = Some v.
+
+  Parameter split_smem_set : forall a b c p v b',
+    split a b c ->
+      smem_set p v b = Some b' ->
+      exists a', split a' b' c /\
+        smem_set p v a = Some a'.
 
 End SeparationMemory.
 
