src/SepLemma.v
@@ -94,3 +94,39 @@ Section typed.
   Proof. clear; induction es; simpl; intuition. Qed.
 
 End typed.
+
+
+Module SepLemma (SE : SepExpr).
+
+  Section typed.
+    Variable types : list type.
+    
+    Definition sepConcl : Type :=
+      (SE.sexpr types * SE.sexpr types)%type.
+
+    Definition Lhs (l : lemma types sepConcl) : SE.sexpr types :=
+      fst (Concl l).
+    Definition Rhs (l : lemma types sepConcl) : SE.sexpr types :=
+      snd (Concl l).
+    
+    Definition WellTyped_sepConcl tfuncs tpreds (vars : list tvar) (c : sepConcl) : bool :=
+      if SE.WellTyped_sexpr tfuncs tpreds nil vars (fst c)
+      then 
+        SE.WellTyped_sexpr tfuncs tpreds nil vars (snd c)
+      else false.
+
+    Definition sepConclD funcs preds (uvars vars : env types) (c : sepConcl) : Prop :=
+      SE.himp funcs preds uvars vars (fst c) (snd c).
+
+    Definition sepLemma : Type := lemma types sepConcl.
+
+    Definition WellTyped_sepLemma tfuncs tpreds (l : sepLemma) : bool :=
+      WellTyped_lemma (WellTyped_sepConcl tfuncs tpreds) tfuncs l.
+
+    Definition sepLemmaD (funcs : functions types) (preds : SE.predicates types) 
+      (meta_base var_base : env types) (lem : sepLemma) : Prop :=
+      lemmaD (WellTyped_sepConcl (typeof_funcs funcs) (SE.typeof_preds preds)) 
+             (sepConclD funcs preds) funcs meta_base var_base lem.
+  End typed.
+
+End SepLemma.
