examples/UsingTheCanceler.v
@@ -1,0 +1,183 @@
+Require Import Bedrock.SepTheory.
+Require Import RelationClasses.
+
+Module SimpleSepLog <: SepTheory_Kernel.
+  Require Import FunctionalExtensionality.
+
+  Definition heap := nat -> option nat.
+
+  Definition hprop := heap -> Prop.
+
+  Definition himp (l r : hprop) : Prop :=
+    forall h, l h -> r h.
+
+  Definition heq (l r : hprop) : Prop :=
+    forall h, l h <-> r h.
+
+  Global Instance Refl_himp : Reflexive himp.
+  Proof. repeat red; intuition. Qed.
+
+  Global Instance Trans_himp : Transitive himp.
+  Proof. repeat red; intuition. Qed.
+
+  Global Instance Refl_heq : Reflexive heq.
+  Proof. repeat red; intuition. Qed.
+
+  Global Instance Sym_heq : Symmetric heq.
+  Proof. repeat red; firstorder. Qed.
+
+  Global Instance Trans_heq : Transitive heq.
+  Proof. repeat red; firstorder. Qed.
+
+  Theorem heq_defn : forall l r, (himp l r /\ himp r l) <-> heq l r.
+  Proof. unfold himp, heq; firstorder. Qed.
+
+  Definition inj (p : Prop) : hprop := fun m => p /\ forall p, m p = None.
+
+  Definition emp : hprop := inj True.
+
+  Definition split (h hl hr : heap) : Prop :=
+    forall p, (hl p = None \/ hr p = None) /\
+      h p = match hl p with
+              | None => hr p
+              | Some x => Some x
+            end.
+              
+  Definition star (l r : hprop) : hprop :=
+    fun h => 
+      exists h1 h2, split h h1 h2 /\
+        l h1 /\ r h2.
+      
+  Definition ex (T : Type) (p : T -> hprop) : hprop :=
+    fun h => exists x, p x h.
+
+  Ltac doIt := 
+    unfold heq, himp, star, emp, split, ex, inj; intros;
+    repeat match goal with 
+             | [ H : exists x, _ |- _ ] => destruct H
+             | [ H : _ /\ _ |- _ ] => destruct H
+           end.
+  
+  Theorem himp_star_comm : forall P Q : hprop, himp (star P Q) (star Q P).
+  Proof.
+    doIt. do 2 eexists; doIt. split. 2: eauto.
+    intro. specialize (H p). intuition; rewrite H in *.
+    destruct (x0 p); auto.
+    destruct (x p); auto.
+  Qed.
+
+  Theorem heq_star_assoc :
+    forall P Q R : hprop, heq (star (star P Q) R) (star P (star Q R)).
+  Proof. 
+    doIt; intuition; doIt.
+    exists x1. exists (fun p => match x2 p with
+                                  | None => x0 p
+                                  | Some x => Some x
+                                end); intuition.
+    specialize (H p); specialize (H0 p); intuition; doIt.
+    rewrite H0 in *. rewrite H4 in *. destruct (x1 p); eauto.
+    rewrite H0 in *; rewrite H4 in *. auto.
+    specialize (H p); specialize (H0 p); intuition;
+    rewrite H0 in *; rewrite H4 in *; eauto.
+    rewrite <- H6 in *; auto.
+    destruct (x1 p); auto; congruence.
+    rewrite H6 in *; auto.
+    destruct (x1 p); auto. destruct (x p); eauto; try congruence.
+    rewrite H6 in *; auto.
+    
+    exists x2. exists x0. intuition.
+    specialize (H p); specialize (H0 p); intuition; doIt.
+    rewrite H0 in *; rewrite H4 in *; auto.
+
+    { exists (fun p => match x p with
+                         | Some x => Some x
+                         | None => x1 p 
+                       end). exists x2.
+      intuition; doIt; try specialize (H p); try specialize (H1 p); intuition;
+        try rewrite H1 in *; try rewrite H4 in *; auto; try congruence.
+      destruct (x p); eauto; congruence.
+      destruct (x p); eauto; congruence.
+      exists x; exists x1; intuition; doIt.
+      specialize (H p); specialize (H1 p); intuition.
+      rewrite H1 in *; rewrite H4 in *.
+      destruct (x1 p); auto. }
+  Qed.
+
+  Theorem heq_star_emp_l : forall P : hprop, heq (star emp P) P.
+  Proof.
+    doIt. intuition; doIt.
+    cutrewrite (h = x0); auto.
+
+    eapply functional_extensionality; intros.
+    specialize (H x1). specialize (H2 x1). rewrite H2 in *. intuition.
+    exists (fun _ => None). exists h. intuition.
+  Qed.
+
+   Theorem himp_subst_p :
+     forall P Q R S : hprop,
+     himp P S -> himp (star S Q) R -> himp (star P Q) R.
+   Proof.
+     doIt. eapply H0; clear H0. do 2 eexists. split; [ | eauto ].
+     intuition.
+   Qed.
+
+   Theorem himp_subst_c :
+     forall P Q R S : hprop,
+     himp S Q -> himp P (star S R) -> himp P (star Q R).
+   Proof.
+     doIt. eapply H0 in H1; clear H0. doIt.
+     do 2 eexists; split; [ | eauto ]. intuition.
+   Qed.
+
+   Theorem himp_star_pure_p :
+     forall (P Q : hprop) (F : Prop),
+     himp (star (inj F) P) Q -> F -> himp P Q.
+   Proof.
+     doIt. eapply H. exists (fun _ => None). exists h.
+     intuition.
+   Qed.
+
+   Theorem himp_star_pure_c :
+     forall (P Q : hprop) (F : Prop),
+     (F -> himp P Q) -> himp (star (inj F) P) Q.
+   Proof.
+     doIt. eapply H; auto.
+     cutrewrite (h = x0); auto.
+     eapply functional_extensionality; intros.
+     specialize (H3 x1). specialize (H0 x1).
+     rewrite H3 in *. intuition.
+   Qed.
+
+   Theorem himp_star_pure_cc :
+     forall (P Q : hprop) (p : Prop),
+     p -> himp P Q -> himp P (star (inj p) Q).
+   Proof.
+     doIt. eapply H0 in H1; clear H0.
+     exists (fun _ => None). exists h.
+     intuition.
+   Qed.
+
+   Theorem himp_ex_p :
+     forall (T : Type) (P : T -> hprop) (Q : hprop),
+     (forall v : T, himp (P v) Q) -> himp (ex T P) Q.
+   Proof.
+     doIt. eauto.
+   Qed.
+       
+   Theorem himp_ex_c :
+     forall (T : Type) (P : T -> hprop) (Q : hprop),
+     (exists v : T, himp Q (P v)) -> himp Q (ex T P).
+   Proof.
+     doIt; eauto.
+   Qed.
+     
+   Theorem heq_ex_star :
+     forall (T : Type) (P : T -> hprop) (Q : hprop),
+     heq (star (ex T P) Q) (ex T (fun x : T => star (P x) Q)).
+   Proof.
+     doIt; intuition; doIt. exists x1.
+     exists x. exists x0. intuition.
+     exists x0. exists x1. intuition. eauto.
+   Qed.
+
+End SimpleSepLog.
